theories/proto/involutive.v
@@ -1,4 +1,0 @@
-From iris.heap_lang Require Import proofmode notation.
-
-Class Involutive {A} (R : relation A) (f : A → A) :=
-  involutive x : R (f (f x)) x.
