theories/proto/side.v
@@ -1,9 +1,0 @@
-From iris.heap_lang Require Import proofmode notation.
-From osiris.proto Require Export involutive.
-
-Inductive side := Left | Right.
-Instance side_inhabited : Inhabited side := populate Left.
-Definition dual_side (s : side) : side :=
-  match s with Left => Right | Right => Left end.
-Instance dual_side_involutive : Involutive (=) dual_side.
-Proof. by intros []. Qed.
