theories/channel/proto_channel.v
@@ -1,0 +1,475 @@
+From osiris.channel Require Export channel.
+From osiris.channel Require Import proto_model.
+From iris.base_logic.lib Require Import invariants.
+From iris.heap_lang Require Import proofmode notation.
+From iris.algebra Require Import auth excl.
+From osiris.utils Require Import auth_excl.
+
+(** Camera setup *)
+Class proto_chanG Σ := {
+  proto_chanG_chanG :> chanG Σ;
+  proto_chanG_authG :> auth_exclG (laterO (proto val (iPreProp Σ) (iPreProp Σ))) Σ;
+}.
+
+Definition proto_chanΣ := #[
+  chanΣ;
+  GFunctor (authRF(optionURF (exclRF (laterOF (protoOF val idOF idOF)))))
+].
+Instance subG_chanΣ {Σ} : subG proto_chanΣ Σ → proto_chanG Σ.
+Proof. intros [??%subG_auth_exclG]%subG_inv. constructor; apply _. Qed.
+
+(** Types and constructors *)
+Definition iProto Σ := proto val (iProp Σ) (iProp Σ).
+Definition iProto_cont Σ X := X -t> val * iProp Σ * iProto Σ.
+
+Delimit Scope proto_scope with proto.
+Bind Scope proto_scope with iProto.
+Delimit Scope proto_cont_scope with proto_cont.
+Bind Scope proto_cont_scope with iProto_cont.
+
+Definition iProto_end {Σ} : iProto Σ := proto_end.
+Program Definition iProto_message {Σ X} (a : action) (pc : iProto_cont Σ X) : iProto Σ :=
+  proto_message a (λ v, λne f, ∃ x : X,
+    ⌜ (tele_app pc x).1.1 = v ⌝ ∗ (tele_app pc x).1.2 ∗ f (Next (tele_app pc x).2))%I.
+Next Obligation. solve_proper. Qed.
+Arguments iProto_message {_ _} _ _%proto_cont.
+
+Definition proto_exist {Σ A} {X : A → tele}
+  (pc : ∀ x : A, iProto_cont Σ (X x)) : iProto_cont Σ (TeleS X) := pc.
+Arguments proto_exist {_ _ _} _%proto.
+Definition proto_payload {Σ} (w : val) (P : iProp Σ)
+  (p : iProto Σ) : iProto_cont Σ TeleO := (w,P,p).
+Arguments proto_payload {_} _%V _%I _%proto.
+
+Notation "<!> pc" := (iProto_message Send pc)
+  (at level 20, pc at level 200) : proto_scope.
+Notation "<?> pc" := (iProto_message Receive pc)
+  (at level 20, pc at level 200) : proto_scope.
+Notation "∃ x .. y , pc" :=
+  (proto_exist (λ x, .. (proto_exist (λ y, pc)) ..)%proto_cont) : proto_cont_scope.
+
+Notation "'MSG' v {{ P }}; p" :=
+  (proto_payload v P p) (at level 20, v at level 20, P, p at level 200) : proto_cont_scope.
+Notation "'MSG' v ; p" :=
+  (proto_payload v True p) (at level 20, v at level 20, p at level 200) : proto_cont_scope.
+
+Definition proto_dual {Σ} (p : iProto Σ) : iProto Σ :=
+  proto_map action_dual cid cid p.
+Arguments proto_dual {_} _%proto.
+
+Class IsActionDual (a1 a2 : action) :=
+  is_action_dual : action_dual a1 = a2.
+Instance is_action_dual_default a : IsActionDual a (action_dual a) | 100 := eq_refl.
+Instance is_action_dual_Send : IsActionDual Send Receive := eq_refl.
+Instance is_action_dual_Receive : IsActionDual Receive Send := eq_refl.
+
+Class IsProtoDual {Σ} (p1 p2 : iProto Σ) :=
+  is_dual_proto : proto_dual p1 ≡ p2.
+Class IsProtoContDual {Σ X} (pc1 pc2 : iProto_cont Σ X) :=
+  is_dual_proto_cont x : prod_map id proto_dual (tele_app pc1 x) ≡ tele_app pc2 x.
+
+(** Invariants *)
+Fixpoint proto_eval `{!proto_chanG Σ} (vs : list val) (p1 p2 : iProto Σ) : iProp Σ :=
+  match vs with
+  | [] => p1 ≡ proto_dual p2
+  | v :: vs => ∃ pc p2',
+     p2 ≡ (proto_message Receive pc)%proto ∗
+     (∀ f : laterO (iProto Σ) -n> iProp Σ, f (Next p2') -∗ pc v f) ∗
+     ▷ proto_eval vs p1 p2'
+  end%I.
+Arguments proto_eval {_ _} _ _%proto _%proto : simpl nomatch.
+
+Record proto_name := ProtName {
+  proto_c_name : chan_name;
+  proto_l_name : gname;
+  proto_r_name : gname
+}.
+
+Definition to_proto_auth_excl `{!proto_chanG Σ} (p : iProto Σ) :=
+  to_auth_excl (Next (proto_map id iProp_fold iProp_unfold p)).
+
+Definition proto_own_frag `{!proto_chanG Σ} (γ : proto_name) (s : side)
+    (p : iProto Σ) : iProp Σ :=
+  own (side_elim s proto_l_name proto_r_name γ) (◯ to_proto_auth_excl p)%I.
+
+Definition proto_own_auth `{!proto_chanG Σ} (γ : proto_name) (s : side)
+    (p : iProto Σ) : iProp Σ :=
+  own (side_elim s proto_l_name proto_r_name γ) (● to_proto_auth_excl p)%I.
+
+Definition proto_inv `{!proto_chanG Σ} (γ : proto_name) : iProp Σ :=
+  (∃ l r pl pr,
+    chan_own (proto_c_name γ) Left l ∗
+    chan_own (proto_c_name γ) Right r ∗
+    proto_own_auth γ Left pl ∗
+    proto_own_auth γ Right pr ∗
+    ▷ ((⌜r = []⌝ ∗ proto_eval l pl pr) ∨
+       (⌜l = []⌝ ∗ proto_eval r pr pl)))%I.
+
+Definition proto_interp `{!proto_chanG Σ, !heapG Σ} (N : namespace)
+    (c : val) (p : iProto Σ) : iProp Σ :=
+  (∃ s (c1 c2 : val) γ,
+    ⌜ c = side_elim s c1 c2 ⌝ ∗
+    proto_own_frag γ s p ∗ is_chan N (proto_c_name γ) c1 c2 ∗ inv N (proto_inv γ))%I.
+Arguments proto_interp {_ _ _} _ _ _%proto.
+Instance: Params (@proto_interp) 5 := {}.
+
+Notation "c ↣ p @ N" := (proto_interp N c p)
+  (at level 20, N at level 50, format "c  ↣  p  @  N").
+
+Section proto.
+  Context `{!proto_chanG Σ, !heapG Σ} (N : namespace).
+
+  Global Instance proto_dual_ne : NonExpansive (@proto_dual Σ).
+  Proof. solve_proper. Qed.
+  Global Instance proto_dual_proper : Proper ((≡) ==> (≡)) (@proto_dual Σ).
+  Proof. apply (ne_proper _). Qed.
+  Global Instance proto_dual_involutive : Involutive (≡) (@proto_dual Σ).
+  Proof.
+    intros p. rewrite /proto_dual -proto_map_compose -{2}(proto_map_id p).
+    apply: proto_map_ext=> //. by intros [].
+  Qed.
+  Lemma proto_dual_end : proto_dual (Σ:=Σ) proto_end ≡ proto_end.
+  Proof. by rewrite /proto_dual proto_map_end. Qed.
+  Lemma proto_dual_message a pc :
+    proto_dual (Σ:=Σ) (proto_message a pc)
+    ≡ proto_message (action_dual a) (ofe_morO_map (ofe_morO_map
+        (laterO_map (proto_map action_dual cid cid)) cid) cid ∘ pc).
+  Proof. by rewrite /proto_dual proto_map_message. Qed.
+
+  Global Instance is_proto_dual_default (p : iProto Σ) :
+    IsProtoDual p (proto_dual p) | 100.
+  Proof. by rewrite /IsProtoDual. Qed.
+  Global Instance is_proto_dual_end : IsProtoDual (@iProto_end Σ) iProto_end.
+  Proof. by rewrite /IsProtoDual /iProto_end proto_dual_end. Qed.
+  Global Instance is_proto_dual_message {X} a1 a2 (pc1 pc2 : iProto_cont Σ X) :
+    IsActionDual a1 a2 →
+    IsProtoContDual pc1 pc2 →
+    IsProtoDual (iProto_message a1 pc1) (iProto_message a2 pc2).
+  Proof.
+    rewrite /IsActionDual /IsProtoContDual /IsProtoDual=> <- Hpc.
+    rewrite /iProto_message proto_dual_message. f_equiv=> v f /=. f_equiv=> x.
+    by destruct (Hpc x) as [[-> ->] <-].
+ Qed.
+
+  Global Instance is_proto_cont_dual_payload v P (p1 p2 : iProto Σ) :
+    IsProtoDual p1 p2 →
+    IsProtoContDual (proto_payload v P p1) (proto_payload v P p2).
+  Proof.
+    rewrite /IsProtoDual /IsProtoContDual=> Hp.
+    apply tforall_forall. by rewrite /= Hp.
+  Qed.
+  Global Instance is_proto_cont_dual_exist {A} {X : A → tele}
+      (pc1 pc2 : ∀ x : A, iProto_cont Σ (X x)) :
+    (∀ x, IsProtoContDual (pc1 x) (pc2 x)) →
+    IsProtoContDual (proto_exist pc1) (proto_exist pc2).
+  Proof.
+    rewrite /IsProtoContDual=> Hpc. apply tforall_forall=> /= x'.
+    apply tforall_forall. apply Hpc.
+  Qed.
+
+  Global Instance proto_eval_ne : NonExpansive2 (proto_eval vs).
+  Proof. induction vs; solve_proper. Qed.
+  Global Instance proto_eval_proper vs : Proper ((≡) ==> (≡) ==> (≡)) (proto_eval vs).
+  Proof. apply (ne_proper_2 _). Qed.
+
+  Global Instance to_proto_auth_excl_ne : NonExpansive to_proto_auth_excl.
+  Proof. solve_proper. Qed.
+  Global Instance proto_own_ne γ s : NonExpansive (proto_own_frag γ s).
+  Proof. solve_proper. Qed.
+  Global Instance proto_interp_ne c : NonExpansive (proto_interp N c).
+  Proof. solve_proper. Qed.
+  Global Instance proto_interp_proper c : Proper ((≡) ==> (≡)) (proto_interp N c).
+  Proof. apply (ne_proper _). Qed.
+
+  Lemma proto_own_auth_agree γ s p p' :
+    proto_own_auth γ s p -∗ proto_own_frag γ s p' -∗ ▷ (p ≡ p').
+  Proof.
+    iIntros "Hauth Hfrag".
+    iDestruct (own_valid_2 with "Hauth Hfrag") as "Hvalid".
+    iDestruct (to_auth_excl_valid with "Hvalid") as "Hvalid".
+    iDestruct (bi.later_eq_1 with "Hvalid") as "Hvalid"; iNext.
+    assert (∀ p : iProto Σ,
+      proto_map id iProp_unfold iProp_fold (proto_map id iProp_fold iProp_unfold p) ≡ p) as help.
+    { intros p''. rewrite -proto_map_compose -{2}(proto_map_id p'').
+      apply proto_map_ext=> // pc /=; by rewrite iProp_fold_unfold. }
+    rewrite -{2}(help p). iRewrite "Hvalid". by rewrite help.
+  Qed.
+
+  Lemma proto_own_auth_update γ s p p' p'' :
+    proto_own_auth γ s p -∗ proto_own_frag γ s p' ==∗
+    proto_own_auth γ s p'' ∗ proto_own_frag γ s p''.
+  Proof.
+    iIntros "Hauth Hfrag".
+    iDestruct (own_update_2 with "Hauth Hfrag") as "H".
+    { eapply (auth_update _ _ (to_proto_auth_excl p'') (to_proto_auth_excl p'')).
+      apply option_local_update. by apply exclusive_local_update. }
+    by rewrite own_op.
+  Qed.
+
+  Lemma proto_eval_send v vs pc p1 p2 :
+    proto_eval vs (proto_message Send pc) p2 -∗
+    (∀ f : laterO (iProto Σ) -n> iProp Σ, f (Next p1) -∗ pc v f) -∗
+    proto_eval (vs ++ [v]) p1 p2.
+  Proof.
+    iIntros "Heval Hc". iInduction vs as [|v' vs] "IH" forall (p2); simpl.
+    - iDestruct "Heval" as "#Heval".
+      iExists _, (proto_dual p1). iSplit.
+      { rewrite -{2}(involutive proto_dual p2). iRewrite -"Heval".
+        by rewrite proto_dual_message. }
+      iSplit.
+      { iIntros (f) "Hf /=". by iApply "Hc". }
+      by rewrite involutive.
+    - iDestruct "Heval" as (pc' p2') "(Heq & Hc' & Heval)".
+      iExists pc', p2'. iFrame "Heq Hc'". iNext. iApply ("IH" with "Heval Hc").
+  Qed.
+
+  Lemma proto_eval_recv v vs p1 pc :
+     proto_eval (v :: vs) p1 (proto_message Receive pc) -∗ ∃ p2,
+       (∀ f : laterO (iProto Σ) -n> iProp Σ, f (Next p2) -∗ pc v f) ∗
+       ▷ proto_eval vs p1 p2.
+  Proof.
+    simpl. iDestruct 1 as (pc' p2) "(Heq & Hc & Hp2)". iExists p2. iFrame "Hp2".
+    iDestruct (@proto_message_equivI with "Heq") as "[_ Heq]".
+    iSpecialize ("Heq" $! v). rewrite bi.ofe_morO_equivI.
+    iIntros (f) "Hfp2". iRewrite ("Heq" $! f). by iApply "Hc".
+  Qed.
+
+  Lemma proto_eval_False p pc v vs :
+    proto_eval (v :: vs) p (proto_message Send pc) -∗ False.
+  Proof.
+    simpl. iDestruct 1 as (pc' p2') "[Heq _]".
+    by iDestruct (@proto_message_equivI with "Heq") as "[% _]".
+  Qed.
+
+  Lemma proto_eval_nil p1 p2 : proto_eval [] p1 p2 -∗ p1 ≡ proto_dual p2.
+  Proof. done. Qed.
+
+  Arguments proto_eval : simpl never.
+
+  Lemma proto_init E cγ c1 c2 p :
+    is_chan N cγ c1 c2 -∗
+    chan_own cγ Left [] -∗ chan_own cγ Right [] ={E}=∗
+    c1 ↣ p @ N ∗ c2 ↣ proto_dual p @ N.
+  Proof.
+    iIntros "#Hcctx Hcol Hcor".
+    iMod (own_alloc (● (to_proto_auth_excl p) ⋅
+                     ◯ (to_proto_auth_excl p))) as (lγ) "[Hlsta Hlstf]".
+    { by apply auth_both_valid_2. }
+    iMod (own_alloc (● (to_proto_auth_excl (proto_dual p)) ⋅
+                     ◯ (to_proto_auth_excl (proto_dual p)))) as (rγ) "[Hrsta Hrstf]".
+    { by apply auth_both_valid_2. }
+    pose (ProtName cγ lγ rγ) as pγ.
+    iMod (inv_alloc N _ (proto_inv pγ) with "[-Hlstf Hrstf Hcctx]") as "#Hinv".
+    { iNext. rewrite /proto_inv. eauto 10 with iFrame. }
+    iModIntro. iSplitL "Hlstf".
+    - iExists Left, c1, c2, pγ; iFrame; auto.
+    - iExists Right, c1, c2, pγ; iFrame; auto.
+  Qed.
+
+  Lemma proto_send_acc {X} E c (pc : iProto_cont Σ X) :
+    ↑N ⊆ E →
+    c ↣ <!> pc @ N -∗ ∃ s c1 c2 γ,
+      ⌜ c = side_elim s c1 c2 ⌝ ∗
+      is_chan N (proto_c_name γ) c1 c2 ∗ |={E,E∖↑N}=> ∃ vs,
+        chan_own (proto_c_name γ) s vs ∗
+        ▷ ∀ (x : X),
+           (tele_app pc x).1.2 -∗
+           chan_own (proto_c_name γ) s (vs ++ [(tele_app pc x).1.1]) ={E∖↑N,E}=∗
+           c ↣ (tele_app pc x).2 @ N.
+  Proof.
+    iIntros (?). iDestruct 1 as (s c1 c2 γ ->) "[Hstf #[Hcctx Hinv]]".
+    iExists s, c1, c2, γ. iSplit; first done. iFrame "Hcctx".
+    iInv N as (l r pl pr) "(>Hclf & >Hcrf & Hstla & Hstra & Hinv')" "Hclose".
+    (* TODO: refactor to avoid twice nearly the same proof *)
+    iModIntro. destruct s.
+    - iExists _.
+      iIntros "{$Hclf} !>" (x) "HP Hclf".
+      iRename "Hstf" into "Hstlf".
+      iDestruct (proto_own_auth_agree with "Hstla Hstlf") as "#Heq".
+      iMod (proto_own_auth_update _ _ _ _ (tele_app pc x).2
+        with "Hstla Hstlf") as "[Hstla Hstlf]".
+      iMod ("Hclose" with "[-Hstlf]") as "_".
+      { iNext. iExists _,_,_,_. iFrame "Hcrf Hstra Hstla Hclf". iLeft.
+        iRewrite "Heq" in "Hinv'".
+        iDestruct "Hinv'" as "[[-> Heval]|[-> Heval]]".
+        { iSplit=> //. iApply (proto_eval_send with "Heval [HP]").
+          iIntros (f) "Hf /=". iExists x. by iFrame. }
+        destruct r as [|vr r]; last first.
+        { iDestruct (proto_eval_False with "Heval") as %[]. }
+        iSplit; first done; simpl. iRewrite (proto_eval_nil with "Heval").
+        iApply (proto_eval_send _ [] with "[] [HP]").
+        { by rewrite /proto_eval involutive. }
+        iIntros (f) "Hf /=". iExists x. by iFrame. }
+      iModIntro. iExists Left, c1, c2, γ. iFrame; auto.
+    - iExists _.
+      iIntros "{$Hcrf} !>" (x) "HP Hcrf".
+      iRename "Hstf" into "Hstrf".
+      iDestruct (proto_own_auth_agree with "Hstra Hstrf") as "#Heq".
+      iMod (proto_own_auth_update _ _ _ _ (tele_app pc x).2
+        with "Hstra Hstrf") as "[Hstra Hstrf]".
+      iMod ("Hclose" with "[-Hstrf]") as "_".
+      { iNext. iExists _, _, _, _. iFrame "Hcrf Hstra Hstla Hclf". iRight.
+        iRewrite "Heq" in "Hinv'".
+        iDestruct "Hinv'" as "[[-> Heval]|[-> Heval]]"; last first.
+        { iSplit=> //. iApply (proto_eval_send with "Heval [HP]").
+          iIntros (f) "Hf /=". iExists x. by iFrame. }
+        destruct l as [|vl l]; last first.
+        { iDestruct (proto_eval_False with "Heval") as %[]. }
+        iSplit; first done; simpl. iRewrite (proto_eval_nil with "Heval").
+        iApply (proto_eval_send _ [] with "[] [HP]").
+        { by rewrite /proto_eval involutive. }
+        iIntros (f) "Hf /=". iExists x. by iFrame. }
+      iModIntro. iExists Right, c1, c2, γ. iFrame; auto.
+  Qed.
+
+  Lemma proto_recv_acc {X} E c (pc : iProto_cont Σ X) :
+    ↑N ⊆ E →
+    c ↣ <?> pc @ N -∗ ∃ s c1 c2 γ,
+      ⌜ c = side_elim s c2 c1 ⌝ ∗
+      is_chan N (proto_c_name γ) c1 c2 ∗ |={E,E∖↑N}=> ∃ vs,
+        chan_own (proto_c_name γ) s vs ∗
+        ▷ ((chan_own (proto_c_name γ) s vs ={E∖↑N,E}=∗
+             c ↣ <?> pc @ N) ∧
+           (∀ v vs',
+             ⌜ vs = v :: vs' ⌝ -∗
+             chan_own (proto_c_name γ) s vs' ={E∖↑N,E}=∗ ▷ ∃ x : X,
+             ⌜ v = (tele_app pc x).1.1 ⌝ ∗
+             ▷ c ↣ (tele_app pc x).2 @ N ∗
+             (tele_app pc x).1.2)).
+  Proof.
+    iIntros (?). iDestruct 1 as (s c1 c2 γ ->) "[Hstf #[Hcctx Hinv]]".
+    iExists (side_elim s Right Left), c1, c2, γ. iSplit; first by destruct s.
+    iFrame "Hcctx".
+    iInv N as (l r pl pr) "(>Hclf & >Hcrf & Hstla & Hstra & Hinv')" "Hclose".
+    iExists (side_elim s r l). iModIntro.
+    (* TODO: refactor to avoid twice nearly the same proof *)
+    destruct s; simpl.
+    - iIntros "{$Hcrf} !>".
+      iRename "Hstf" into "Hstlf".
+      iDestruct (proto_own_auth_agree with "Hstla Hstlf") as "#Heq".
+      iSplit.
+      + iIntros "Hown".
+        iMod ("Hclose" with "[-Hstlf]") as "_".
+        { iNext. iExists l, r, _, _. iFrame. }
+        iModIntro. iExists Left, c1, c2, γ. by iFrame "Hcctx ∗ Hinv".
+      + iIntros (v vs ->) "Hown".
+        iDestruct "Hinv'" as "[[>% _]|[> -> Heval]]"; first done.
+        iAssert (▷ proto_eval (v :: vs) pr (<?> pc))%I with "[Heval]" as "Heval".
+        { iNext. by iRewrite "Heq" in "Heval". }
+        iDestruct (proto_eval_recv with "Heval") as (q) "[Hf Heval]".
+        iMod (proto_own_auth_update _ _ _ _ q with "Hstla Hstlf") as "[Hstla Hstlf]".
+        iMod ("Hclose" with "[-Hstlf Hf]") as %_.
+        { iExists _, _,_ ,_. eauto 10 with iFrame. }
+        iIntros "!> !>".
+        set (f p := (∃ q, p ≡ Next q ∧ c1 ↣ q @ N)%I).
+        assert (NonExpansive f) by solve_proper.
+        iDestruct ("Hf" $! (OfeMor f) with "[Hstlf]") as (x <-) "[HP Hf] /=".
+        { iExists q. iSplit; first done. iExists Left, c1, c2, γ. iFrame; auto. }
+        iExists x. iSplit; first done. iFrame "HP".
+        iDestruct "Hf" as (q') "[#Hq Hc]". iModIntro. by iRewrite "Hq".
+    - iIntros "{$Hclf} !>".
+      iRename "Hstf" into "Hstrf".
+      iDestruct (proto_own_auth_agree with "Hstra Hstrf") as "#Heq".
+      iSplit.
+      + iIntros "Hown".
+        iMod ("Hclose" with "[-Hstrf]") as "_".
+        { iNext. iExists l, r, _, _. iFrame. }
+        iModIntro. iExists Right, c1, c2, γ. by iFrame "Hcctx ∗ Hinv".
+      + iIntros (v vs ->) "Hown".
+        iDestruct "Hinv'" as "[[>-> Heval]|[>% _]]"; last done.
+        iAssert (▷ proto_eval (v :: vs) pl (<?> pc))%I with "[Heval]" as "Heval".
+        { iNext. by iRewrite "Heq" in "Heval". }
+        iDestruct (proto_eval_recv with "Heval") as (q) "[Hf Heval]".
+        iMod (proto_own_auth_update _ _ _ _ q with "Hstra Hstrf") as "[Hstra Hstrf]".
+        iMod ("Hclose" with "[-Hstrf Hf]") as %_.
+        { iExists _, _, _, _. eauto 10 with iFrame. }
+        iIntros "!> !>".
+        set (f p := (∃ q, p ≡ Next q ∧ c2 ↣ q @ N)%I).
+        assert (NonExpansive f) by solve_proper.
+        iDestruct ("Hf" $! (OfeMor f) with "[Hstrf]") as (x <-) "[HP Hf] /=".
+        { iExists q. iSplit; first done. iExists Right, c1, c2, γ. iFrame; auto. }
+        iExists x. iSplit; first done. iFrame "HP".
+        iDestruct "Hf" as (q') "[#Hq Hc]". iModIntro. by iRewrite "Hq".
+  Qed.
+
+  Lemma new_chan_proto_spec p1 p2 :
+    IsProtoDual p1 p2 →
+    {{{ True }}}
+      new_chan #()
+    {{{ c1 c2, RET (c1,c2); c1 ↣ p1 @ N ∗ c2 ↣ p2 @ N }}}.
+  Proof.
+    rewrite /IsProtoDual.
+    iIntros (Hp2 Ψ _) "HΨ". iApply wp_fupd. wp_apply new_chan_spec=> //.
+    iIntros (c1 c2 γ) "(Hc & Hl & Hr)".
+    iMod (proto_init ⊤ γ c1 c2 p1 with "Hc Hl Hr") as "[Hp Hdp]".
+    iApply "HΨ". rewrite -Hp2. by iFrame.
+  Qed.
+
+  Lemma send_proto_spec_packed {X} c (pc : iProto_cont Σ X) (x : X) :
+    {{{ c ↣ <!> pc @ N ∗ (tele_app pc x).1.2 }}}
+      send c (tele_app pc x).1.1
+    {{{ RET #(); c ↣ (tele_app pc x).2 @ N }}}.
+  Proof.
+    iIntros (Ψ) "[Hp Hf] HΨ".
+    iDestruct (proto_send_acc ⊤ with "Hp") as (γ s c1 c2 ->) "[#Hc Hvs]"; first done.
+    iApply (send_spec with "[$]"). iMod "Hvs" as (vs) "[Hch H]".
+    iModIntro. iExists vs. iFrame "Hch".
+    iIntros "!> Hvs". iApply "HΨ".
+    iMod ("H" $! x with "Hf Hvs"); auto.
+  Qed.
+
+  Lemma send_proto_spec {X} Ψ c v (pc : iProto_cont Σ X) :
+    c ↣ <!> pc @ N -∗
+    (∃.. x : X,
+      ⌜ v = (tele_app pc x).1.1 ⌝ ∗
+      (tele_app pc x).1.2 ∗
+      (c ↣ (tele_app pc x).2 @ N -∗ Ψ #())) -∗
+    WP send c v {{ Ψ }}.
+  Proof.
+    iIntros "Hc H". iDestruct (bi_texist_exist with "H") as (x ->) "[HP HΨ]".
+    by iApply (send_proto_spec_packed with "[$]").
+  Qed.
+
+  Lemma try_recv_proto_spec_packed {X} c (pc : iProto_cont Σ X) :
+    {{{ c ↣ <?> pc @ N }}}
+      try_recv c
+    {{{ v, RET v; (⌜v = NONEV⌝ ∧ c ↣ <?> pc @ N) ∨
+                  (∃ x : X, ⌜v = SOMEV ((tele_app pc x).1.1)⌝ ∗
+                            c ↣ (tele_app pc x).2 @ N ∗ (tele_app pc x).1.2) }}}.
+  Proof.
+    iIntros (Ψ) "Hp HΨ".
+    iDestruct (proto_recv_acc ⊤ with "Hp") as (γ s c1 c2 ->) "[#Hc Hvs]"; first done.
+    wp_apply (try_recv_spec with "[$]"). iSplit.
+    - iMod "Hvs" as (vs) "[Hch [H _]]".
+      iIntros "!> !>". iMod ("H" with "Hch") as "Hch". iApply "HΨ"; auto.
+    - iMod "Hvs" as (vs) "[Hch [_ H]]".
+      iIntros "!>". iExists vs. iIntros "{$Hch} !>" (v vs' ->) "Hch".
+      iMod ("H" with "[//] Hch") as "H"; iIntros "!> !>".
+      iDestruct "H" as (x ->) "H". iIntros "!>". iApply "HΨ"; auto.
+  Qed.
+
+  Lemma recv_proto_spec_packed {X} c (pc : iProto_cont Σ X) :
+    {{{ c ↣ <?> pc @ N }}}
+      recv c
+    {{{ x, RET (tele_app pc x).1.1;
+        c ↣ (tele_app pc x).2 @ N ∗ (tele_app pc x).1.2 }}}.
+  Proof.
+    iIntros (Ψ) "Hp HΨ".
+    iDestruct (proto_recv_acc ⊤ with "Hp") as (γ s c1 c2 ->) "[#Hc Hvs]"; first done.
+    wp_apply (recv_spec with "[$]"). iMod "Hvs" as (vs) "[Hch [_ H]]".
+    iModIntro. iExists vs. iFrame "Hch". iIntros "!>" (v vs' ->) "Hvs'".
+    iMod ("H" with "[//] Hvs'") as "H"; iIntros "!> !>".
+    iDestruct "H" as (x ->) "H". iIntros "!>". by iApply "HΨ".
+  Qed.
+
+  Lemma recv_proto_spec {X} Ψ c (pc : iProto_cont Σ X) :
+    c ↣ <?> pc @ N -∗
+    (∀.. x : X, c ↣ (tele_app pc x).2 @ N -∗
+                (tele_app pc x).1.2 -∗ Ψ (tele_app pc x).1.1) -∗
+    WP recv c {{ Ψ }}.
+  Proof.
+    iIntros "Hc H". iApply (recv_proto_spec_packed with "[$]").
+    iIntros "!>" (x) "[Hc HP]". iDestruct (bi_tforall_forall with "H") as "H".
+    iApply ("H" with "[$] [$]").
+  Qed.
+End proto. 
