theories/utils/auth_excl.v
@@ -1,7 +1,6 @@
-From iris.heap_lang Require Export lang.
 From iris.proofmode Require Import tactics.
 From iris.algebra Require Import excl auth.
-From iris.base_logic.lib Require Import auth.
+From iris.base_logic.lib Require Import own.
 Set Default Proof Using "Type".
 
 Class auth_exclG (A : ofeT) (Σ : gFunctors) := AuthExclG {
